Modularising IMM

src/basic/FinExecution.v
@@ -5,16 +5,23 @@ From hahnExt Require Import HahnExt.
 Require Import Events.
 Require Import Execution.
 
-Notation "'Tid_' t" := (fun x => tid x = t) (at level 1).
+Module FinExecution
+    (Val : ValueSig)
+    (Ev : Events Val).
+
+Module Import Ex := Execution Val Ev.
+
+Notation "'Tid_' t" := (fun x => Ev.tid x = t) (at level 1).
 
 Definition fin_exec (G: execution) :=
-  set_finite (acts_set G \₁ is_init).
+  set_finite (Ex.acts_set G \₁ Ev.is_init).
 
 Definition fin_exec_full (G: execution) :=
-  set_finite (acts_set G).
+  set_finite (Ex.acts_set G).
 
 Lemma fin_exec_full_equiv (G: execution):
-  fin_exec_full G <-> fin_exec G /\ set_finite (acts_set G ∩₁ is_init).
+  fin_exec_full G <->
+  fin_exec G /\ set_finite (Ex.acts_set G ∩₁ Ev.is_init).
 Proof using.
   unfold fin_exec, fin_exec_full.
   rewrite <- set_finite_union. apply set_finite_more. 
@@ -22,26 +29,27 @@ Proof using.
   basic_solver.
 Qed. 
 
-Section FinExecution.
+Section FinExecutionDefs.
   Variable G: execution.
 
   Hypothesis FINDOM: fin_exec_full G.
 
   Lemma exists_nE thread :
-    exists n, ~ acts_set G (ThreadEvent thread n).
+    exists n, ~ Ex.acts_set G (Ev.ThreadEvent thread n).
   Proof using FINDOM.
     set (AA:=FINDOM).
-    apply set_finite_exists_bigger with (f:=ThreadEvent thread) in AA.
+    apply set_finite_exists_bigger with (f:=Ev.ThreadEvent thread) in AA.
     3: { ins. desf. }
-    2: { apply eq_dec_actid. }
+    2: { apply Ev.eq_dec_actid. }
     desf.
     exists (1 + n). apply AA. lia.
   Qed.
 
-  Definition acts_list: list actid :=
-    filterP (acts_set G \₁ is_init)
+  Definition acts_list: list Ev.actid :=
+    filterP (Ex.acts_set G \₁ Ev.is_init)
             (proj1_sig (@constructive_indefinite_description _ _ FINDOM)).
-  Lemma acts_set_findom: acts_set G \₁ is_init ≡₁ (fun e => In e acts_list).
+  Lemma acts_set_findom:
+    Ex.acts_set G \₁ Ev.is_init ≡₁ (fun e => In e acts_list).
   Proof using.
     unfold acts_list. destruct constructive_indefinite_description. simpl.
     split; intros e.
@@ -49,22 +57,24 @@ Section FinExecution.
     apply i. apply H.
   Qed.
   Opaque acts_list.
-End FinExecution. 
+End FinExecutionDefs.
 
 Lemma fin_exec_same_events G G'
-      (SAME: acts_set G ≡₁ acts_set G') (FIN: fin_exec G):
+      (SAME: Ex.acts_set G ≡₁ Ex.acts_set G') (FIN: fin_exec G):
   fin_exec G'.
 Proof using. unfold fin_exec in *. by rewrite <- SAME. Qed.
 
-Lemma tid_is_init_fin_helper (S: actid -> Prop) thread
-      (NT: thread <> tid_init)
-      (FIN: set_finite (S \₁ is_init)):
+Lemma tid_is_init_fin_helper (S: Ev.actid -> Prop) thread
+      (NT: thread <> Ev.tid_init)
+      (FIN: set_finite (S \₁ Ev.is_init)):
   set_finite (S ∩₁ Tid_ thread).
 Proof using. 
-  rewrite set_split_complete with (s := is_init).
+  rewrite set_split_complete with (s := Ev.is_init).
   apply set_finite_union. split.
   { eapply set_finite_mori; [| by apply set_finite_empty].
     red. unfolder. ins. desc. vauto. by destruct x. }
   eapply set_finite_mori; [| by apply FIN].
   red. basic_solver.
 Qed. 
+
+End FinExecution.
