src/basic/FairExecution.v
@@ -7,29 +7,37 @@ Require Import Execution.
 Import ListNotations.
 Require Import FinExecution.
 
-Definition mem_fair (G: execution) := fsupp (co G) /\ fsupp (fr G). 
+Module FairExecution
+    (Val : ValueSig)
+    (Ev : Events Val).
 
-Section FairExecution.
+Module Import Fin := FinExecution Val Ev.
+Module Import Ex := Fin.Ex.
+
+Definition mem_fair (G: execution) :=
+  fsupp (Ex.co G) /\ fsupp (Ex.fr G). 
+
+Section FairExecutionDefs.
   Variable G: execution.
   Hypothesis FAIR: mem_fair G.
   Hypothesis WF: Wf G. 
 
   Lemma co_imm:
-    co G ≡ (immediate (co G))⁺.
+    Ex.co G ≡ (immediate (Ex.co G))⁺.
   Proof using WF FAIR. apply fsupp_imm_t; apply WF || apply FAIR. Qed. 
 
   Lemma nS_imm_co_in_sb
-        (S : actid -> Prop) w wnext
-        (WW : is_w (lab G) w)
+        (S : Ev.actid -> Prop) w wnext
+        (WW : Ev.is_w (Ex.lab G) w)
         (NSW : ~ S w)
-        (NCOIMM : immediate ((co G) ⨾ ⦗S⦘) w wnext)
-        (FOR_SPLIT : ⦗set_compl S⦘ ⨾ immediate (co G) ⊆ sb G) :
-    sb G w wnext.
+        (NCOIMM : immediate ((Ex.co G) ⨾ ⦗S⦘) w wnext)
+        (FOR_SPLIT : ⦗set_compl S⦘ ⨾ immediate (Ex.co G) ⊆ Ex.sb G) :
+    Ex.sb G w wnext.
   Proof using WF FAIR.
-    assert (transitive (co G)) as COTRANS.
+    assert (transitive (Ex.co G)) as COTRANS.
     { apply (co_trans WF). }
 
-    assert (S wnext /\ co G w wnext) as [ISSNEXT CONEXT].
+    assert (S wnext /\ Ex.co G w wnext) as [ISSNEXT CONEXT].
     { generalize NCOIMM. basic_solver. }
     apply clos_trans_of_transitiveD; [apply sb_trans|].
     apply (inclusion_t_t FOR_SPLIT).
@@ -41,7 +49,7 @@ Section FairExecution.
     apply t_rt_step. exists z; split; [|apply seq_eqv_l; split; [|done]].
     { apply rtE in IMMS. destruct IMMS as [IMMS|IMMS].
       { red in IMMS; desf. apply rt_refl. }
-      assert (immediate ((co G) ⨾ ⦗S⦘) z wnext) as IMM'.
+      assert (immediate ((Ex.co G) ⨾ ⦗S⦘) z wnext) as IMM'.
       { red; split; [apply seq_eqv_r; split; auto|].
         { (* TODO: is the last tactic needed? *)
           apply clos_trans_immediate1; auto; try by apply ct_step. }
@@ -53,13 +61,13 @@ Section FairExecution.
       clear IMM.
       induction IMMS.
       { apply rt_step. apply seq_eqv_l; split; auto. }
-      assert (co G y wnext) as YNEXT.
+      assert (Ex.co G y wnext) as YNEXT.
       { apply clos_trans_immediate1; auto.
         eapply transitive_ct; [by apply IMMS2|].
         eapply same_relation_exp.
         { symmetry. apply fsupp_imm_t; apply FAIR || apply WF. }
         unfolder in IMM'. basic_solver. }
-      assert (immediate ((co G) ⨾ ⦗S⦘) y wnext) as YNEXTIMM.
+      assert (immediate ((Ex.co G) ⨾ ⦗S⦘) y wnext) as YNEXTIMM.
       { red; split; [by apply seq_eqv_r; split|].
         ins. eapply NCOIMM; [|by apply R2].
         apply seq_eqv_r in R1; destruct R1 as [R1 R3].
@@ -83,66 +91,68 @@ Section FairExecution.
     all: by apply ct_step.
   Qed.
   
-  Lemma fsupp_rf: fsupp (rf G).
+  Lemma fsupp_rf: fsupp (Ex.rf G).
   Proof using WF.
     apply functional_inv_fsupp. by inversion WF.
   Qed.
 
   Lemma fsupp_sb:
-    fsupp (⦗set_compl is_init⦘ ⨾ sb G).
+    fsupp (⦗set_compl Ev.is_init⦘ ⨾ Ex.sb G).
   Proof using WF.
-    unfold sb, ext_sb; unfolder; ins.
+    unfold Ex.sb, Ev.ext_sb; unfolder; ins.
     destruct y; [exists nil; ins; desf|].
-    exists (map (fun i => ThreadEvent thread i) (List.seq 0 index)).
+    exists (map (fun i => Ev.ThreadEvent thread i) (List.seq 0 index)).
     intros e ((NIe & E0) & (SB & E)).
     destruct e; [done| ]. destruct SB as [-> LT].
     apply in_map_iff. eexists. split; eauto. by apply in_seq0_iff.
   Qed.
 
   Lemma fsupp_sb_loc:
-    fsupp (sb G ∩ same_loc (lab G)).
+    fsupp (Ex.sb G ∩ Ev.same_loc (Ex.lab G)).
   Proof using WF.
     rewrite <- seq_id_l.
-    rewrite set_full_split with (S := is_init), id_union, seq_union_l.
+    rewrite set_full_split with (S := Ev.is_init), id_union, seq_union_l.
     apply fsupp_union.
     2: { eapply fsupp_mori; [| by apply fsupp_sb; eauto].
          red. basic_solver. }
     
     red. ins.
-    remember (loc (lab G) y) as ly. destruct ly. 
-    { exists [InitEvent l].
+    remember (Ev.loc (Ex.lab G) y) as ly. destruct ly. 
+    { exists [Ev.InitEvent l].
       intros x REL%seq_eqv_l. desc. destruct x; [| done].
       simpl. left. f_equal. apply proj2 in REL0.
       red in REL0.
-      unfold Events.loc in REL0 at 1. rewrite wf_init_lab in REL0; auto.
+      unfold Ev.loc in REL0 at 1. rewrite wf_init_lab in REL0; auto.
       congruence. }
     exists []. red. intros x REL%seq_eqv_l. desc.
     apply proj2 in REL0. red in REL0.
     destruct x; [| done]. 
-    unfold Events.loc in REL0 at 1. rewrite wf_init_lab in REL0; auto.
+    unfold Ev.loc in REL0 at 1. rewrite wf_init_lab in REL0; auto.
     congruence.
   Qed.
   
   
-End FairExecution.
+End FairExecutionDefs.
 
 Lemma fin_exec_fair G (WF: Wf G) (FIN: fin_exec G):
   mem_fair G.
 Proof using.
   red. apply fsupp_union_iff.
-  arewrite (co G ∪ fr G ≡ ⦗acts_set G⦘ ⨾ (co G ∪ fr G) ⨾ ⦗is_w (lab G)⦘).
+  arewrite (Ex.co G ∪ Ex.fr G ≡
+            ⦗Ex.acts_set G⦘ ⨾ (Ex.co G ∪ Ex.fr G) ⨾
+            ⦗Ev.is_w (Ex.lab G)⦘).
   { rewrite wf_coE, wf_frE, wf_coD, wf_frD; eauto. basic_solver 10. }
   red. intros w.
-  destruct (classic (is_w (lab G) w)) as [W | NW].
+  destruct (classic (Ev.is_w (Ex.lab G) w)) as [W | NW].
   2: { exists []. intros. apply seq_eqv_lr in REL. by desc. }
-  forward eapply is_w_loc as [l Lw]; eauto. 
+  forward eapply Ev.is_w_loc as [l Lw]; eauto. 
   destruct FIN as [findom FIN].
-  exists (InitEvent l :: findom).
+  exists (Ev.InitEvent l :: findom).
   intros r REL%seq_eqv_lr. desc.
   destruct r eqn:RR.
   { simpl. left. f_equal. eapply hahn_inclusion_exp in REL0.
     2: { rewrite wf_col, wf_frl, unionK; eauto. reflexivity. }
-    red in REL0. unfold loc in REL0 at 1. rewrite wf_init_lab in REL0; auto.
+    red in REL0. unfold Ev.loc in REL0 at 1. rewrite wf_init_lab in REL0; auto.
     congruence. }
   right. apply FIN. split; auto. 
 Qed. 
@@ -152,3 +162,5 @@ Lemma fin_exec_full_fair G (WF: Wf G) (FIN: fin_exec_full G):
 Proof using.
   apply fin_exec_fair; auto. apply fin_exec_full_equiv in FIN. by desc. 
 Qed. 
+
+End FairExecution.
