src/basic/ProgToExecution.v
@@ -1,4 +1,4 @@
-Require Import RelationClasses List Lia.
+(* Require Import RelationClasses List Lia.
 From hahn Require Import Hahn.
 From PromisingLib Require Import Loc.
 Require Import Events.
@@ -344,4 +344,4 @@ Section State.
     all: unfold upd; desf.
   Qed.
 
-End State.
+End State. *)
