src/imm/imm_common_more.v
@@ -13,56 +13,64 @@ Require Import imm_bob.
 
 Set Implicit Arguments.
 
-Section IMM.
+Module imm_common_more (Val : ValueSig) (Ev : Events Val).
+
+Module Import Ppo := imm_s_ppo Val Ev.
+Module Import SHb := Ppo.SHb.
+Module Import Bob := SHb.Bob.
+Module Import Eco := Bob.Eco.
+Module Import Ex := Eco.Ex.
+
+Section ImmCommonMoreDefs.
 
 Variable G : execution.
 
-Notation "'E'" := (acts_set G).
-Notation "'sb'" := (sb G).
-Notation "'rf'" := (rf G).
-Notation "'co'" := (co G).
-Notation "'rmw'" := (rmw G).
-Notation "'data'" := (data G).
-Notation "'addr'" := (addr G).
-Notation "'ctrl'" := (ctrl G).
-Notation "'rmw_dep'" := (rmw_dep G).
+Notation "'E'" := (Ex.acts_set G).
+Notation "'sb'" := (Ex.sb G).
+Notation "'rf'" := (Ex.rf G).
+Notation "'co'" := (Ex.co G).
+Notation "'rmw'" := (Ex.rmw G).
+Notation "'data'" := (Ex.data G).
+Notation "'addr'" := (Ex.addr G).
+Notation "'ctrl'" := (Ex.ctrl G).
+Notation "'rmw_dep'" := (Ex.rmw_dep G).
 
-Notation "'fr'" := (fr G).
-Notation "'eco'" := (eco G).
-Notation "'coe'" := (coe G).
-Notation "'coi'" := (coi G).
-Notation "'deps'" := (deps G).
-Notation "'rfi'" := (rfi G).
-Notation "'rfe'" := (rfe G).
-Notation "'detour'" := (detour G).
-Notation "'fwbob'" := (fwbob G).
-Notation "'bob'" := (bob G).
-Notation "'ppo'" := (ppo G).
-Notation "'ar_int'" := (ar_int G).
+Notation "'fr'" := (Ex.fr G).
+Notation "'eco'" := (Eco.eco G).
+Notation "'coe'" := (Ex.coe G).
+Notation "'coi'" := (Ex.coi G).
+Notation "'deps'" := (Ex.deps G).
+Notation "'rfi'" := (Ex.rfi G).
+Notation "'rfe'" := (Ex.rfe G).
+Notation "'detour'" := (Ex.detour G).
+Notation "'fwbob'" := (Bob.fwbob G).
+Notation "'bob'" := (Bob.bob G).
+Notation "'ppo'" := (Ppo.ppo G).
+Notation "'ar_int'" := (Ppo.ar_int G).
 
-Notation "'lab'" := (lab G).
-Notation "'loc'" := (loc lab).
-Notation "'val'" := (val lab).
-Notation "'mod'" := (mod lab).
-Notation "'same_loc'" := (same_loc lab).
+Notation "'lab'" := (Ex.lab G).
+Notation "'loc'" := (Ev.loc lab).
+Notation "'val'" := (Ev.val lab).
+Notation "'mod'" := (Ev.mod lab).
+Notation "'same_loc'" := (Ev.same_loc lab).
 
-Notation "'R'" := (fun a => is_true (is_r lab a)).
-Notation "'W'" := (fun a => is_true (is_w lab a)).
-Notation "'F'" := (fun a => is_true (is_f lab a)).
+Notation "'R'" := (fun a => is_true (Ev.is_r lab a)).
+Notation "'W'" := (fun a => is_true (Ev.is_w lab a)).
+Notation "'F'" := (fun a => is_true (Ev.is_f lab a)).
 Notation "'RW'" := (R ∪₁ W).
 Notation "'FR'" := (F ∪₁ R).
 Notation "'FW'" := (F ∪₁ W).
-Notation "'R_ex'" := (R_ex G).
-Notation "'W_ex'" := (W_ex G).
-Notation "'W_ex_acq'" := (W_ex ∩₁ (fun a => is_true (is_xacq lab a))).
+Notation "'R_ex'" := (fun a => is_true (Ev.R_ex lab a)).
+Notation "'W_ex'" := (Ex.W_ex G).
+Notation "'W_ex_acq'" := (W_ex ∩₁ (fun a => is_true (Ev.is_xacq lab a))).
 
-Notation "'Pln'" := (fun a => is_true (is_only_pln lab a)).
-Notation "'Rlx'" := (fun a => is_true (is_rlx lab a)).
-Notation "'Rel'" := (fun a => is_true (is_rel lab a)).
-Notation "'Acq'" := (fun a => is_true (is_acq lab a)).
-Notation "'Acqrel'" := (fun a => is_true (is_acqrel lab a)).
-Notation "'Acq/Rel'" := (fun a => is_true (is_ra lab a)).
-Notation "'Sc'" := (fun a => is_true (is_sc lab a)).
+Notation "'Pln'" := (fun a => is_true (Ev.is_only_pln lab a)).
+Notation "'Rlx'" := (fun a => is_true (Ev.is_rlx lab a)).
+Notation "'Rel'" := (fun a => is_true (Ev.is_rel lab a)).
+Notation "'Acq'" := (fun a => is_true (Ev.is_acq lab a)).
+Notation "'Acqrel'" := (fun a => is_true (Ev.is_acqrel lab a)).
+Notation "'Acq/Rel'" := (fun a => is_true (Ev.is_ra lab a)).
+Notation "'Sc'" := (fun a => is_true (Ev.is_sc lab a)).
 
 (******************************************************************************)
 (** ** Derived relations  *)
@@ -88,7 +96,7 @@ assert (helper:
 ∪ sb ⨾ ⦗F ∩₁ Acq/Rel⦘ ∪ detour ⨾ (⦗R∩₁Acq⦘ ⨾ sb)^? ∪ ppo ∪ ⦗W_ex_acq⦘ ⨾ sb ⨾ ⦗W⦘ ∪ ⦗W_ex⦘ ⨾ rfi ⨾ ⦗R∩₁Acq⦘ ⨾ sb^?)＊).
 by apply inclusion_rt_rt; basic_solver 12.
 
-unfold imm_s_ppo.ar_int, imm_bob.bob, imm_bob.fwbob.
+unfold Ppo.ar_int, Bob.bob, Bob.fwbob.
 
 arewrite (sb ⨾ ⦗W ∩₁ Rel⦘ ∪ ⦗W ∩₁ Rel⦘ ⨾ sb ∩ same_loc ⨾ ⦗W⦘ ∪ sb ⨾ ⦗F ∩₁ Acq/Rel⦘
  ∪ ⦗F ∩₁ Acq/Rel⦘ ⨾ sb ∪ ⦗R ∩₁ Acq⦘ ⨾ sb ∪ ppo ∪ detour
@@ -189,10 +197,10 @@ generalize (@sb_trans G); ins; relsf.
 Qed.
 
 Lemma W_sb_same_loc_detour WF (SC_PER_LOC: sc_per_loc G) :
-⦗fun x => ~ is_init x⦘ ⨾ ⦗W⦘ ⨾ sb ∩ same_loc ⨾ ⦗W⦘ ⨾ detour ⊆ detour.
+⦗fun x => ~ Ev.is_init x⦘ ⨾ ⦗W⦘ ⨾ sb ∩ same_loc ⨾ ⦗W⦘ ⨾ detour ⊆ detour.
 Proof using.
 sin_rewrite (w_sb_loc_w_in_coi WF SC_PER_LOC).
-unfold Execution.detour. 
+unfold Ex.detour. 
 unfolder; ins; desf.
 splits.
 - exists z0; splits; eauto.
@@ -241,7 +249,7 @@ arewrite_id ⦗W⦘ at 1.
 generalize (@sb_trans G); ins; relsf.
 basic_solver 12.
 * rewrite !seqA.
-arewrite (⦗W ∩₁ Rel⦘ ⊆ ⦗fun x => ~ is_init x⦘ ⨾ ⦗W⦘).
+arewrite (⦗W ∩₁ Rel⦘ ⊆ ⦗fun x => ~ Ev.is_init x⦘ ⨾ ⦗W⦘).
 { unfolder; ins; desf; splits; eauto.
 intro K; apply (init_pln WF) in K; mode_solver. }
 sin_rewrite (W_sb_same_loc_detour WF SC_PER_LOC).
@@ -366,4 +374,6 @@ basic_solver 21.
 Qed.
 
 
-End IMM.
+End ImmCommonMoreDefs.
+
+End imm_common_more.
